builtins for refl typing

src/ocaml-output/FStar_Parser_Const.ml
@@ -526,6 +526,11 @@ let (universe_uvar_lid : FStar_Ident.lident) =
 let (check_with_lid : FStar_Ident.lident) =
   FStar_Ident.lid_of_path ["FStar"; "Reflection"; "Builtins"; "check_with"]
     FStar_Compiler_Range.dummyRange
+let (dsl_typing_builtin : Prims.string -> FStar_Ident.lident) =
+  fun s ->
+    FStar_Ident.lid_of_path
+      (FStar_Compiler_List.op_At ["Refl"; "Typing"; "Builtins"] [s])
+      FStar_Compiler_Range.dummyRange
 let (dsl_tac_typ_lid : FStar_Ident.lident) =
   FStar_Ident.lid_of_path ["Refl"; "Typing"; "dsl_tac_t"]
     FStar_Compiler_Range.dummyRange
