src/tactics/FStar.Tactics.Basic.fsti
@@ -116,3 +116,8 @@ val comp_to_string         : comp -> tac string
 
 val term_eq_old            : term -> term -> tac bool
 val with_compat_pre_core   : Z.t -> tac 'a -> tac 'a
+
+(*****)
+val refl_check_subtyping : env -> typ -> typ -> tac (option unit)
+val refl_check_equiv     : env -> typ -> typ -> tac (option unit)
+val refl_tc_term         : env -> term -> tac (option typ)
